Need to redo parts of Cancel

platform/Depl/Cancel.v
@@ -48,6 +48,7 @@ Ltac t := simpl; intuition;
             | [ H1 : vcs _ -> _, H2 : vcs (_ ++ _) |- _ ] =>
               specialize (H1 (vcs_app_bwd1 _ _ H2)) || specialize (H1 (vcs_app_bwd2 _ _ H2))
             | [ H : exists x, _ |- _ ] => destruct H; intuition
+            | [ _ : context[match ?p with pair _ _ => _ end] |- _ ] => destruct p
           end; simpl in *); eauto.
 
 (** * Substitution *)
@@ -55,15 +56,26 @@ Ltac t := simpl; intuition;
 Definition sub_expr (s : fo_sub) (e : expr) : option expr :=
   match e with
     | Var x => s x
-    | Lift f => Some (Lift f)
+    | Lift f => Some (Lift (fun fE => f (fun x => match s x with
+                                                    | None => Dyn tt
+                                                    | Some e => exprD e fE
+                                                  end)))
   end.
 
-Lemma sub_expr_monotone : forall s s',
-  (forall x e, s x = Some e -> s' x = Some e)
-  -> forall e e', sub_expr s e = Some e'
-    -> sub_expr s' e = Some e'.
+Lemma sub_expr_monotone : forall s s' e,
+  (forall fE fE', (forall x, s x <> None -> fE x = fE' x) -> exprD e fE = exprD e fE')
+  -> (forall x e, s x = Some e -> s' x = Some e)
+  -> forall e', sub_expr s e = Some e'
+    -> exists e'', sub_expr s' e = Some e''
+      /\ forall fE, exprD e' fE = exprD e'' fE.
 Proof.
   destruct e; t.
+  repeat esplit; simpl; intros.
+  apply H; intros.
+  specialize (H0 x).
+  destruct (s x).
+  erewrite H0; eauto.
+  tauto.
 Qed.
 
 Fixpoint sub_exprs (s : fo_sub) (es : list expr) : option (list expr) :=
@@ -104,6 +116,28 @@ Lemma sub_pred_monotone : forall s s',
     -> sub_pred s' p = Some p'.
 Proof.
   destruct p; t; erewrite sub_exprs_monotone; eauto.
+Qed.
+
+Fixpoint sub_preds (s : fo_sub) (ps : list pred) : option (list pred) :=
+  match ps with
+    | nil => Some nil
+    | p :: ps =>
+      match sub_pred s p with
+        | None => None
+        | Some p =>
+          match sub_preds s ps with
+            | None => None
+            | Some ps => Some (p :: ps)
+          end
+      end
+  end.
+
+Lemma sub_preds_monotone : forall s s',
+  (forall x e, s x = Some e -> s' x = Some e)
+  -> forall es es', sub_preds s es = Some es'
+    -> sub_preds s' es = Some es'.
+Proof.
+  induction es; t; erewrite sub_pred_monotone; eauto.
 Qed.
 
 (** * Unification *)
@@ -176,9 +210,6 @@ Local Hint Immediate vcs_app_bwd1 vcs_app_bwd2.
 
 Ltac unify_args := t;
   match goal with
-    | [ _ : context[match ?p with pair _ _ => _ end] |- _ ] => destruct p
-  end;
-  match goal with
     | [ _ : context[unify_args ?s ?lhs ?rhs], IH : forall rhs : list expr, _ |- _ ] =>
       let Heq := fresh in
       specialize (IH rhs s); case_eq (unify_args s lhs rhs); [
@@ -245,9 +276,417 @@ Qed.
 
 (** Result of cancelation *)
 Inductive result :=
-| Success (NewLhs : normal) (ProveThese : list Prop)
+| Success (NewLhs : list pred) (ProveThese : list Prop)
 | Failure (Message : Prop).
 
-(*Fixpoint cancel' (s : fo_sub) (lhs : normal) (p : pred) : result.
+(** Result of canceling just one atomic predicate *)
+Inductive result1 :=
+| Success1 (NewSub : fo_sub) (NewLhs : list pred) (ProveThese : list Prop)
+| Failure1 (Message : Prop).
 
-Definition cancel (lhs rhs : normal) : result.*)
+Inductive noMatchFor (rhs : pred) := .
+
+(** Find a LHS match for a single RHS predicate. *)
+Fixpoint findMatching (s : fo_sub) (lhs : list pred) (rhs : pred) : result1 :=
+  match lhs with
+    | nil => Failure1 (noMatchFor rhs)
+    | p :: lhs =>
+      match unify_pred s p rhs with
+        | Some (s, Ps) => Success1 s lhs Ps 
+        | None =>
+          match findMatching s lhs rhs with
+            | Success1 s lhs Ps => Success1 s (p :: lhs) Ps
+            | x => x
+          end
+      end
+  end.
+
+Local Hint Resolve unify_pred_monotone.
+
+Theorem findMatching_monotone : forall rhs lhs s s' lhs' Ps,
+  findMatching s lhs rhs = Success1 s' lhs' Ps
+  -> forall x e, s x = Some e -> s' x = Some e.
+Proof.
+  induction lhs; t.
+
+  injection H; clear H; intros; subst; eauto.
+
+  specialize (IHlhs s).
+  destruct (findMatching s lhs rhs); try discriminate.
+  injection H; clear H; intros; subst; eauto.
+Qed.
+
+Local Hint Resolve findMatching_monotone.
+
+Theorem findMatching_sound : forall G (hE : ho_env G) S fE rhs lhs s s' lhs' Ps,
+  findMatching s lhs rhs = Success1 s' lhs' Ps
+  -> vcs Ps
+  -> exists rhs', sub_pred s' rhs = Some rhs'
+    /\ (SubstsH S (fold_left (fun hp p => starB (predD p hE fE) hp) lhs (empB _))
+    ===> SubstsH S (predD rhs' hE fE)
+    * SubstsH S (fold_left (fun hp p => starB (predD p hE fE) hp) lhs' (empB _))).
+Proof.
+  induction lhs; t.
+
+  match goal with
+    | [ H : Success1 _ _ _ = Success1 _ _ _ |- _ ] => injection H; clear H; intros; subst
+  end.
+  eapply unify_pred_sound in H1; eauto; t.
+  repeat esplit.
+  eapply Himp_trans; [ apply star_out_fwd | ].
+  apply SubstsH_star_fwd.
+
+  match goal with
+    | [ _ : context[findMatching ?s ?lhs ?rhs], IH : forall s : fo_sub, _ |- _ ] =>
+      let Heq := fresh in specialize (IH s); case_eq (findMatching s lhs rhs);
+        [ intros ? ? ? Heq; rewrite Heq in *; specialize (IH _ _ _ eq_refl)
+          | intros ? Heq; rewrite Heq in *; try discriminate ]
+  end.
+  match goal with
+    | [ H : Success1 _ _ _ = Success1 _ _ _ |- _ ] => injection H; clear H; intros; subst
+  end.
+  t.
+  repeat esplit.
+
+  eapply Himp_trans; [ apply star_out_fwd | ].
+  eapply Himp_trans; [ apply SubstsH_star_fwd | ].
+  eapply Himp_trans; [ | apply Himp_star_frame; [ apply Himp_refl | apply star_out_bwd ] ].
+  eapply Himp_trans; [ | apply Himp_star_frame; [ apply Himp_refl | apply SubstsH_star_bwd ] ].
+  eapply Himp_trans; [ | apply Himp_star_assoc ].
+  eapply Himp_trans; [ | apply Himp_star_frame; [ apply Himp_star_comm | apply Himp_refl ] ].
+  eapply Himp_trans; [ | apply Himp_star_assoc' ].
+  apply Himp_star_frame; auto; apply Himp_refl.
+Qed.
+
+(** Find LHS matches for all RHS predicates. *)
+Fixpoint findMatchings (s : fo_sub) (lhs rhs : list pred) : result1 :=
+  match rhs with
+    | nil => Success1 s lhs nil
+    | p :: rhs =>
+      match findMatching s lhs p with
+        | Success1 s lhs Ps =>
+          match findMatchings s lhs rhs with
+            | Success1 s lhs Ps' => Success1 s lhs (Ps ++ Ps')
+            | x => x
+          end
+        | x => x
+      end
+  end.
+
+Theorem findMatchings_monotone : forall rhs lhs s s' lhs' Ps,
+  findMatchings s lhs rhs = Success1 s' lhs' Ps
+  -> forall x e, s x = Some e -> s' x = Some e.
+Proof.
+  induction rhs; t.
+
+  case_eq (findMatching s lhs a); intros.
+  rewrite H1 in *.
+  specialize (IHrhs NewLhs NewSub).
+  destruct (findMatchings NewSub NewLhs rhs); try discriminate.
+  injection H; clear H; intros; subst.
+  eauto.
+
+  rewrite H1 in *; discriminate.
+Qed.
+
+Local Hint Resolve findMatchings_monotone.
+
+Theorem findMatchings_sound : forall G (hE : ho_env G) S fE rhs lhs s s' lhs' Ps,
+  findMatchings s lhs rhs = Success1 s' lhs' Ps
+  -> vcs Ps
+  -> exists rhs', sub_preds s' rhs = Some rhs'
+    /\ (SubstsH S (fold_left (fun hp p => starB (predD p hE fE) hp) lhs (empB _))
+    ===> SubstsH S (fold_left (fun hp p => starB (predD p hE fE) hp) rhs' (empB _))
+    * SubstsH S (fold_left (fun hp p => starB (predD p hE fE) hp) lhs' (empB _))).
+Proof.
+  induction rhs; t.
+
+  injection H; clear H; intros; subst.
+  repeat esplit.
+  eapply Himp_trans; [ | apply Himp_star_frame; [ apply SubstsH_emp_bwd | apply Himp_refl ] ].
+  apply Himp_star_Emp'.
+
+  match goal with
+    | [ _ : context[findMatching ?s ?lhs ?rhs] |- _ ] =>
+      let Heq := fresh in case_eq (findMatching s lhs rhs); [ intros ? ? ? Heq | intros ? Heq ];
+        rewrite Heq in *; try discriminate
+  end.
+  match goal with
+    | [ _ : context[findMatchings ?s ?lhs ?rhs], IH : forall lhs : list pred, _ |- _ ] =>
+      let Heq := fresh in specialize (IH lhs s); case_eq (findMatchings s lhs rhs);
+        [ intros ? ? ? Heq; rewrite Heq in *; specialize (IH _ _ _ eq_refl)
+          | intros ? Heq; rewrite Heq in *; try discriminate ]
+  end.
+  match goal with
+    | [ H : Success1 _ _ _ = Success1 _ _ _ |- _ ] => injection H; clear H; intros; subst
+  end; t.
+  specialize (findMatching_sound _ hE S fE _ _ _ _ _ _ H1); t.
+  erewrite sub_pred_monotone; [ .. | eauto ]; eauto.
+  repeat esplit.
+  eapply Himp_trans; [ apply H6 | ].
+  simpl.
+  eapply Himp_trans; [ | apply Himp_star_frame; [ apply star_out_bwd | apply Himp_refl ] ].
+  eapply Himp_trans; [ | apply Himp_star_frame; [ apply SubstsH_star_bwd | apply Himp_refl ] ].
+  eapply Himp_trans; [ | apply Himp_star_assoc' ].
+  apply Himp_star_frame; auto; apply Himp_refl.
+Qed.
+
+(** Overall cancelation *)
+Definition cancel (lhs rhs : normal) : result :=
+  match findMatchings fos_empty (NImpure lhs) (NImpure rhs) with
+    | Failure1 msg => Failure msg
+    | Success1 s lhs' Ps => Success lhs' (
+      (forall x, In x (NQuants rhs) -> s x <> None)
+      :: match NPure rhs with
+           | None => Ps
+           | Some P =>
+             (forall fE1 fE2, (forall x, s x <> None -> fE1 x = fE2 x)
+               -> P fE1 = P fE2)
+             :: (forall fE,
+               let fE' := (fun x => match s x with
+                                      | None => Dyn tt
+                                      | Some e => exprD e fE
+                                    end) in
+               match NPure lhs with
+                 | None => P fE'
+                 | Some P1 => P1 fE -> P fE'
+               end)
+             :: Ps
+         end)
+  end.
+
+Theorem cancel_sound : forall fE G (hE : ho_env G) S lhs rhs lhs' Ps,
+  cancel lhs rhs = Success lhs' Ps
+  -> vcs Ps
+  -> SubstsH S (normalD lhs hE fE)
+  ===> SubstsH S (normalD rhs hE fE)
+  * SubstsH S (normalD {| NQuants := NQuants lhs;
+    NPure := None;
+    NImpure := lhs' |} hE fE).
+Proof.
+  unfold cancel; intros.
+  
+  case_eq (findMatchings fos_empty (NImpure lhs) (NImpure rhs)); intros.
+  Focus 2.
+  rewrite H1 in *; discriminate.
+
+  rewrite H1 in *.
+  injection H; clear H; intros; subst.
+  inversion H0; clear H0; intros; subst.
+  assert (vcs ProveThese) by t.
+  specialize (fun fE => findMatchings_sound _ hE S fE _ _ _ _ _ _ H1); intro Hfms.
+  eapply Himp_trans; [ | apply Himp_star_comm ].
+
+  Lemma addQuants_gulp : forall G (f : _ -> hpropB G) S p qs fE,
+    SubstsH S (addQuants qs (fun fE => f fE * p) fE)
+    ===> SubstsH S (addQuants qs f fE) * SubstsH S p.
+  Proof.
+    induction qs; t.
+
+    apply SubstsH_star_fwd.
+
+    eapply Himp_trans; [ apply SubstsH_ex_fwd | ].
+    apply Himp'_ex; intro.
+    eapply Himp_trans; [ apply IHqs | ].
+    apply Himp_star_frame; try apply Himp_refl.
+    eapply Himp_trans; [ | apply SubstsH_ex_bwd ].
+    apply Himp_ex_c; eauto.
+    eexists; apply Himp_refl.
+  Qed.
+
+  eapply Himp_trans; [ | apply addQuants_gulp ].
+  simpl.
+  apply addQuants_monotone; intros.
+  specialize (Hfms fE'); intuition.
+  destruct H2; intuition.
+  eapply Himp_trans; [ apply multistar_weaken | ].
+  instantiate (1 := (match NPure lhs with
+                       | Some P => [|P fE'|]
+                       | None => Emp
+                     end * Emp)%Sep).
+  eapply Himp_trans; [ | apply SubstsH_star_bwd ].
+  eapply Himp_trans; [ | apply Himp_star_frame; [ apply Himp_refl | apply SubstsH_emp_bwd ] ].
+  eapply Himp_trans; [ | apply Himp_star_comm ].
+  apply Himp_star_Emp'.
+  eapply Himp_trans; [ apply star_out_fwd | ].
+  eapply Himp_trans; [ apply SubstsH_star_fwd | ].
+  eapply Himp_trans; [ apply Himp_star_frame; [ apply Himp_refl | apply H6 ] | ].
+  eapply Himp_trans; [ | apply SubstsH_star_bwd ].
+  eapply Himp_trans; [ apply Himp_star_assoc' | ].
+  eapply Himp_trans; [ apply Himp_star_comm | ].
+  apply Himp_star_frame; try apply Himp_refl.
+  
+  Lemma sub_expr_closed : forall s e,
+    (forall fE fE', exprD e fE = exprD e fE')
+    -> forall e', sub_expr s e = Some e'
+      -> e' = e.
+  Proof.
+    destruct e; simpl; intuition.
+    exfalso.
+    specialize (H (fun _ => Dyn tt) (fun _ => Dyn false)).
+    assert (forall x y : unit, x = y).
+    destruct x0, y; auto.
+    simpl in *.
+    apply (f_equal Ty) in H; simpl in *.
+    rewrite H in H1.
+    specialize (H1 true false); discriminate.
+  Qed.
+
+  Lemma sub_pred_closed : forall s p,
+    wellScoped nil p
+    -> forall p', sub_pred s p = Some p'
+      -> p' = p.
+  Proof.
+    destruct p; simpl; intuition.
+    case_eq (sub_exprs s es); intros.
+    Focus 2.
+    rewrite H1 in H0; discriminate.
+    rewrite H1 in H0; injection H0; clear H0; intros; subst.
+    f_equal.
+    generalize dependent l.
+    induction es; simpl; intuition.
+    simpl in *.
+    case_eq (sub_expr s a); intros.
+    Focus 2.
+    rewrite H0 in *; discriminate.
+    rewrite H0 in *.
+    apply sub_expr_closed in H0; eauto.
+    subst.
+    case_eq (sub_exprs s es); intros.
+    Focus 2.
+    rewrite H0 in *; discriminate.
+    rewrite H0 in *.
+    injection H1; clear H1; intros; subst.
+    f_equal; eauto.
+    intros; eapply H; auto; tauto.
+  Qed.
+
+  Lemma sub_preds_closed : forall s ps,
+    List.Forall (wellScoped nil) ps
+    -> forall ps', sub_preds s ps = Some ps'
+      -> ps' = ps.
+  Proof.
+    induction 1; simpl; intuition.
+    case_eq (sub_pred s x); intros.
+    Focus 2.
+    rewrite H2 in *; discriminate.
+    rewrite H2 in *.
+    case_eq (sub_preds s l); intros.
+    Focus 2.
+    rewrite H3 in *; discriminate.
+    rewrite H3 in *.
+    injection H1; clear H1; intros; subst.
+    f_equal; auto.
+    eapply sub_pred_closed; eauto.
+  Qed.
+
+  Lemma choose_existentials_expr : forall qs fE fE' s e e',
+    (forall fE fE', (forall x, In x qs -> fE x = fE' x)
+      -> exprD e fE = exprD e fE')
+    -> List.Forall (fun x => exists e, s x = Some e /\ fE x = exprD e fE') qs
+    -> sub_expr s e = Some e'
+    -> exprD e fE' = exprD e' fE.
+  Proof.
+    destruct e; simpl; intuition.
+    Focus 2.
+    injection H1; clear H1; intros; subst.
+    simpl.
+    apply H.
+    intros.
+    eapply Forall_forall in H0; eauto.
+    
+
+  Lemma choose_existentials_exprs : forall qs fE fE' s es es',
+    (forall fE fE', (forall x, In x qs -> fE x = fE' x)
+      -> forall e, In e es -> exprD e fE = exprD e fE')
+    -> List.Forall (fun x => exists e, s x = Some e /\ fE x = exprD e fE') qs
+    -> sub_exprs s es = Some es'
+    -> map (fun e => exprD e fE') es = map (fun e : expr => exprD e fE) es'.
+  Proof.
+    induction es; simpl; intuition.
+
+    injection H1; clear H1; intros; subst; auto.
+
+    case_eq (sub_e
+
+  Lemma choose_existentials_pred : forall G (hE : ho_env G) S qs p p' fE fE' s,
+     wellScoped qs p
+     -> List.Forall (fun x => exists e, s x = Some e /\ fE x = exprD e fE') qs
+     -> sub_pred s p = Some p'
+     -> SubstsH S (predD p hE fE') ===> SubstsH S (predD p' hE fE).
+  Proof.
+    destruct p; simpl; intuition.
+    case_eq (sub_exprs s es); intros.
+    Focus 2.
+    rewrite H2 in *; discriminate.
+    rewrite H2 in *.
+    injection H1; clear H1; intros; subst.
+    simpl.
+    
+
+
+  Lemma choose_existentials : forall G (hE : ho_env G) fE S s ps' qs qs' ps fE',
+    sub_preds s ps = Some ps'
+    -> List.Forall (wellScoped (qs ++ qs')) ps
+    -> List.Forall (fun x => exists e, s x = Some e /\ fE x = exprD e fE') qs'
+    -> SubstsH S (fold_left (fun hp p => predD p hE fE' * hp) ps' Emp)
+    ===> SubstsH S (addQuants qs
+      (fun fE0 => fold_left (fun hp p => predD p hE fE0 * hp) ps Emp) fE).
+  Proof.
+    induction qs; simpl; intuition.
+
+    generalize dependent ps'.
+    induction H0; simpl; intuition.
+    injection H; clear H; intros; subst.
+    apply Himp_refl.
+    case_eq (sub_pred s x); intros.
+    Focus 2.
+    rewrite H3 in H2; discriminate.
+    rewrite H3 in *.
+    case_eq (sub_preds s l); intros.
+    Focus 2.
+    rewrite H4 in *; discriminate.
+    rewrite H4 in *.
+    injection H2; clear H2; intros; subst.
+    simpl.
+    eapply Himp_trans; [ apply star_out_fwd | ].
+    eapply Himp_trans; [ apply SubstsH_star_fwd | ].
+    eapply Himp_trans; [ | apply star_out_bwd ].
+    eapply Himp_trans; [ | apply SubstsH_star_bwd ].
+    apply Himp_star_frame; auto.
+
+
+
+    replace ps' with ps.
+    admit. (*apply Himp_refl.*)
+    symmetry; eapply sub_preds_closed; eauto.
+
+    eapply Himp_trans; [ | apply SubstsH_ex_bwd ].
+    case_eq (s a); intros.
+    2: solve [ exfalso; eauto ].
+    apply Himp_ex_c; exists (exprD e fE).
+    apply IHqs.
+
+
+    
+
+    
+
+  Lemma choose_existentials : forall G (hE : ho_env G) fE S s rhs ps,
+    sub_preds s (NImpure rhs) = Some ps
+    -> match NPure rhs with
+         | None => True
+         | Some P => P fE
+       end
+    -> (forall x T, In (x, T) (NQuants rhs) -> s x <> None)
+    -> SubstsH S (fold_left (fun hp p => predD p hE fE * hp) ps Emp)
+    ===> SubstsH S (normalD rhs hE fE).
+  Proof.
+    unfold normalD.
+    
+  
+  specialize (f
+
+  SearchAbout Himp empB.
+  apply Himp_emp.
+  SearchAbout fold_left SubstsH.
